src/Util/Fin.v
@@ -1,0 +1,356 @@
+Require Import Eqdep_dec.
+Require Import PeanoNat.
+Require List.
+
+Import EqNotations.
+
+
+#[local] Hint Resolve Nat.eq_dec : core.
+
+(* (|T| + n)-valued type *)
+
+Fixpoint n_options (n : nat) (T : Set) : Set :=
+match n with
+| O => T
+| S n => option (n_options n T)
+end.
+
+Module NOptions.
+
+Lemma sum_prop (n m : nat) {T} : n_options n (n_options m T) = n_options (n + m) T.
+Proof. induction n. auto. simpl. apply (f_equal (fun (T : Set) => option T)). apply IHn. Qed.
+
+Corollary S_option (n : nat) {T} : n_options (S n) T = n_options n (option T).
+Proof. symmetry. etransitivity. apply (sum_prop n 1). rewrite Nat.add_1_r. reflexivity. Qed.
+
+Fixpoint is_added {T n} (x : n_options n T) : Prop :=
+match n as n' return n_options n' T -> Prop with
+| 0 => fun _ => False
+| S n => fun x =>
+  match x with
+  | None => True
+  | Some x => is_added x
+  end
+end x.
+
+Lemma is_added_dec {T n} (x : n_options n T) : is_added x + not (is_added x).
+Proof. induction n. eauto. destruct x as [ x | ]; simpl; eauto. Qed.
+
+End NOptions.
+
+
+(* n-valued type *)
+
+Definition fin n := n_options n False.
+
+Module Fin.
+
+Fixpoint to_nat {n} (i : fin n) : nat :=
+match n, i with
+| 0, i => match i with end
+| S n, i =>
+  match i with
+  | None => 0
+  | Some i => S (to_nat i)
+  end
+end.
+
+Lemma to_nat_prop {n} {i : fin n} : to_nat i < n.
+Proof.
+induction n. contradiction. destruct i as [ i | ].
+  * apply -> Nat.succ_lt_mono. apply IHn.
+  * apply Nat.lt_0_succ.
+Qed.
+
+Lemma to_nat_inj {n} (i1 i2 : fin n) (p : to_nat i1 = to_nat i2) : i1 = i2.
+Proof.
+  induction n. contradiction.
+  destruct i1 as [ i1 | ]; destruct i2 as [ i2 | ]; inversion p; auto.
+  f_equal. apply IHn. auto.
+Qed.
+
+Lemma to_nat_rew n m (i : fin n) (p : n = m) : to_nat (rew [fin] p in i) = to_nat i.
+Proof. destruct p. auto. Qed.
+
+Fixpoint of_nat n i (p : i < n) : fin n :=
+match n as n', p return fin n' with
+| 0, p => False_rec _ (match p with end)
+| S n, p =>
+  match i as i' return i' < S n -> fin (S n) with
+  | 0 => fun _ => None
+  | S i => fun p => Some (of_nat n i (PeanoNat.lt_S_n i n p))
+  end p
+end.
+
+Lemma of_nat_irrelevance n i (p q : i < n) : of_nat n i p = of_nat n i q.
+Proof.
+  generalize dependent i. induction n; intros.
+  - inversion p.
+  - destruct i; auto. apply (f_equal Some). apply IHn.
+Qed.
+
+Lemma of_nat_inj n i j (p : i < n) (q : j < n) (s : of_nat n i p = of_nat n j q) : i = j.
+Proof.
+  generalize dependent i. generalize dependent j.
+  induction n; intros. inversion p. destruct i; destruct j; inversion s. auto.
+  f_equal. unshelve eapply IHn; eauto.
+Qed.
+
+Lemma of_nat_ext n i j (p : i < n) (q : j < n) (s : i = j) : of_nat n i p = of_nat n j q.
+Proof. generalize dependent p. rewrite s. intro. apply of_nat_irrelevance. Qed.
+
+Lemma fin_nat_fin n (i : fin n) : of_nat n (to_nat i) to_nat_prop = i.
+Proof.
+  induction n. contradiction. destruct i; auto.
+  simpl. f_equal. erewrite of_nat_irrelevance. apply IHn.
+Qed.
+
+Lemma nat_fin_nat n i (p : i < n) : to_nat (of_nat n i p) = i.
+Proof.
+  generalize dependent i. induction n; intros. inversion p.
+  destruct i; auto. simpl. f_equal. apply IHn.
+Qed.
+
+Lemma fin_n_m {n m} (p : n = m) {x : fin n} {y : fin m} (q : rew p in x = y) : rew p in x = y.
+Proof. auto. Qed.
+
+Lemma fin_0_0 {n m} (p : S n = S m) : rew [fin] p in (None : fin (S n)) = None.
+Proof. refine (match p with eq_refl => eq_refl end). Qed.
+
+End Fin.
+
+
+(* telescope is like list but types dependent on (|V| + length of tail)-valued type *)
+
+Inductive telescope (T : Set -> Set) V : nat -> Set :=
+| NilTelescope : telescope T V 0
+| ConsTelescope {n} : T (n_options n V) -> telescope T V n -> telescope T V (S n)
+.
+
+Arguments NilTelescope {_ _}.
+Arguments ConsTelescope {_ _ _} _ _.
+
+Module Telescope.
+
+Fixpoint apply {T : Set -> Set} (subst : forall V, T V -> T (option V) -> T V)
+               {V n} (tsc : telescope T V n) (t : T (n_options n V)) : T V :=
+match tsc in telescope _ _ n' return T (n_options n' V) -> T V with
+| NilTelescope => fun t => t
+| ConsTelescope t' tsc => fun t => apply subst tsc (subst _ t' t)
+end t.
+
+Fixpoint collapse {T V n} (tsc : telescope T V n) {U} (v : n_options n U)
+                  : option { m & prod (T (n_options m V)) (telescope T V m) } :=
+match tsc in telescope _ _ n' return n_options n' U -> _ with
+| NilTelescope => fun _ => None
+| ConsTelescope t tsc => fun v =>
+  match v with
+  | None => Some (existT _ _ (t, tsc))
+  | Some v => collapse tsc v
+  end
+end v.
+
+Lemma collapse_some {T V n} (tsc : telescope T V n) {U} (v : n_options n U)
+                    : NOptions.is_added v <-> exists res, collapse tsc v = Some res.
+Proof.
+  constructor; intro; (induction tsc; [ try destruct H; inversion H | destruct v as [ v | ];
+    [ apply IHtsc; auto | ] ]).
+  eexists. reflexivity. constructor.
+Qed.
+
+Lemma collapse_none {T V n} (tsc : telescope T V n) {U} (v : n_options n U)
+                    : ~(NOptions.is_added v) <-> collapse tsc v = None.
+Proof.
+  constructor; intro; (induction tsc; [ | destruct v as [ v | ]; [ apply IHtsc; auto | ] ]); auto.
+  - apply False_rec. apply H. constructor.
+  - inversion H.
+Qed.
+
+Lemma collapse_some_m {T V n} (tsc : telescope T V n) {U} (v : n_options n U)
+                      {m res} (p : collapse tsc v = Some (existT _ m res))
+                      : m < n.
+Proof.
+  generalize dependent m. induction tsc; intros. inversion p. destruct v as [ v | ].
+  apply IHtsc in p. auto. simpl in p. inversion p. auto.
+Qed.
+
+Lemma collapse_compose {T V n} (tsc : telescope T V n)
+                       {U1 U2 m1} (v1 : n_options n U1) (v2 : n_options m1 U2)
+                       {t1 tsc1} (p : collapse tsc v1 = Some (existT _ m1 (t1, tsc1)))
+                       {m2 t2 tsc2} (q : collapse tsc1 v2 = Some (existT _ m2 (t2, tsc2)))
+                       : exists (v : n_options n U2), collapse tsc v = Some (existT _ m2 (t2, tsc2)).
+Proof.
+  induction tsc. inversion p. destruct v1 as [ v1 | ]. simpl in * |-. apply IHtsc in p.
+  destruct p as [ v Hv ]. exists (Some v). apply Hv. simpl in *. inversion p. subst m1.
+  apply inj_pair2_eq_dec in H1; auto. apply inj_pair2_eq_dec in H2; auto. subst t1 tsc1.
+  exists (Some v2). auto.
+Qed.
+
+Lemma apply_collapse {T : Set -> Set} (pure : forall (V : Set), V -> T V)
+                     (subst : forall V, T V -> T (option V) -> T V)
+                     (subst_pure1 : forall (V : Set) (t : T V), subst _ t (pure _ None) = t)
+                     (subst_pure2 : forall (V : Set) (v : V) (t : T V), subst _ t (pure _ (Some v)) = pure _ v)
+                     {V n} (tsc : telescope T V n) (v : n_options n V)
+                     {m t tsc'} (H : collapse tsc v = Some (existT _ m (t, tsc')))
+                     : apply subst tsc (pure _ v) = apply subst tsc' t.
+Proof.
+  generalize dependent m. induction tsc; intros. inversion H. destruct v.
+  etransitivity; [ | apply IHtsc; eauto ]. simpl. rewrite subst_pure2. reflexivity.
+  simpl. rewrite subst_pure1. inversion H. subst m. specialize Nat.eq_dec. intro.
+  apply inj_pair2_eq_dec in H2; auto. apply inj_pair2_eq_dec in H3; auto.
+  subst t0 tsc'. reflexivity.
+Qed.
+
+Lemma apply_not_added {T : Set -> Set} (pure : forall (V : Set), V -> T V)
+                      (subst : forall V, T V -> T (option V) -> T V)
+                      (subst_pure : forall (V : Set) (v : V) (t : T V), subst _ t (pure _ (Some v)) = pure _ v)
+                      {V n} (tsc : telescope T V n) (v : n_options n V) (H : ~(NOptions.is_added v))
+                      : exists v', apply subst tsc (pure _ v) = pure _ v'.
+Proof.
+  induction tsc. eexists. reflexivity. simpl. destruct v as [ v | ].
+  destruct (IHtsc v); eauto. rewrite subst_pure. rewrite H0. eexists. reflexivity.
+  exfalso. apply H. constructor.
+Qed.
+
+End Telescope.
+
+
+(* [n] -> T ≈ list of n values, but not inductive *)
+
+Definition array (T : Set) n : Set := fin n -> T.
+
+Module Array.
+
+(*
+(* dependent version requires funext :( *)
+Fixpoint array_rec {T R : Set} (z : R) (s : T -> R -> R) n (xs : array T n) : R :=
+match n as n' return array T n' -> R with
+| 0 => fun _ => z
+| S n => fun xs => s (xs None) (array_rec z s n (fun i => xs (Some i)))
+end xs.
+
+Definition to_list {T} {n} (xs : array T n) : list T :=
+  array_rec nil cons n xs.
+
+Fixpoint of_list {T : Set} (xs : list T) : array T (length xs) :=
+match xs as xs' return array T (length xs') with
+| nil => fun i => match i with end
+| cons x xs => fun i =>
+  match i with
+  | None => x
+  | Some i => of_list xs i
+  end
+end.
+
+Definition take {t} [n] i (p : i <= n) (xs : array t n) : array t i :=
+  fun j => xs (Fin.of_nat n (Fin.to_nat j) (Nat.lt_le_trans _ i n Fin.to_nat_prop p)).
+
+Lemma array_take_irrelevance {t n} i (p q : i <= n) (xs : array t n) (j : fin i)
+                             : take i p xs j = take i q xs j.
+Proof. unfold take. f_equal. apply Fin.of_nat_irrelevance. Qed.
+*)
+
+Definition in_array {t : Set} {n} (x : t) (xs : array t n) := exists i, xs i = x.
+
+End Array.
+
+
+(* vector - list of n values *)
+
+Inductive vec (T : Set) : nat -> Set :=
+| NilVec : vec T 0
+| ConsVec : forall {n}, T -> vec T n -> vec T (S n)
+.
+
+Arguments NilVec {_}.
+Arguments ConsVec {_} [_] _ _.
+
+Module Vec.
+
+Fixpoint v2a {T n} (xs : vec T n) : array T n :=
+match xs as xs' in vec _ n' return array T n' with
+| NilVec => fun i => match i with end
+| ConsVec x xs => fun i =>
+  match i with
+  | None => x
+  | Some i => v2a xs i
+  end
+end.
+
+(* essentialy this is definitely "fun i => f (v2a xs i)"
+   but works as workaround on termination checker *)
+Fixpoint v2a_dep {T : Set} [R : T -> Type] (f : forall x, R x)
+                 {n} (xs : vec T n) : forall (i : fin n), R (v2a xs i) :=
+match xs as xs' in vec _ n' return forall (i : fin n'), R (v2a xs' i) with
+| NilVec => fun i => match i with end
+| ConsVec x xs => fun i =>
+  match i as i' return R (v2a (ConsVec x xs) i') with
+  | None => f x
+  | Some i => v2a_dep f xs i
+  end
+end.
+
+Lemma v2a_dep_prop {T : Set} [R : T -> Type] (f : forall x, R x)
+                   {n} (xs : vec T n) (i : fin n)
+                   : v2a_dep f xs i = f (v2a xs i).
+Proof. induction xs. inversion i. destruct i. apply IHxs. auto. Qed.
+
+Fixpoint a2v {T n} (xs : array T n) : vec T n :=
+match n as n' return array T n' -> vec T n' with
+| 0 => fun _ => NilVec
+| S n => fun xs => ConsVec (xs None) (a2v (fun i => xs (Some i)))
+end xs.
+
+Lemma a2v_ext {T n} [xs ys : array T n] (H : forall i, xs i = ys i) : a2v xs = a2v ys.
+Proof. induction n. auto. simpl. f_equal; auto. Qed.
+
+Lemma vec_array_vec {T n} (xs : vec T n) : a2v (v2a xs) = xs.
+Proof. induction xs. auto. simpl. f_equal. auto. Qed.
+
+Lemma array_vec_array {T n} (xs : array T n) (i : fin n) : v2a (a2v xs) i = xs i.
+Proof. induction n. inversion i. destruct i. apply IHn. auto. Qed.
+
+Fixpoint map {T R : Set} (f : T -> R) {n} (xs : vec T n) : vec R n :=
+match xs in vec _ n' return vec R n' with
+| NilVec => NilVec
+| ConsVec x xs => ConsVec (f x) (map f xs)
+end.
+
+Lemma map_prop {T R : Set} (f : T -> R) {n} (xs : vec T n)
+               : map f xs = a2v (fun i => f (v2a xs i)).
+Proof. induction xs. auto. simpl. f_equal. auto. Qed.
+
+Corollary map_id {T n} (xs : vec T n) : map id xs = xs.
+Proof. rewrite map_prop. apply vec_array_vec. Qed.
+
+Corollary map_map {T S R : Set} (f : S -> R) (g : T -> S) {n} (xs : vec T n)
+                  : map f (map g xs) = map (fun x => f (g x)) xs.
+Proof. repeat rewrite map_prop. apply a2v_ext. intro. rewrite array_vec_array. auto. Qed.
+
+Corollary map_ext {T R : Set} [f g : T -> R] {n} (xs : vec T n)
+                  (H : forall i, f (v2a xs i) = g (v2a xs i))
+                  : map f xs = map g xs.
+Proof. repeat rewrite map_prop. apply a2v_ext. auto. Qed.
+
+Definition indices n := a2v (fun (i : fin n) => i).
+
+Fixpoint to_list {T n} (xs : vec T n) : list T :=
+match xs with
+| NilVec => nil
+| ConsVec x xs => cons x (to_list xs)
+end.
+
+Lemma to_list_length {T n} (xs : vec T n) : length (to_list xs) = n.
+Proof. induction xs. auto. simpl. f_equal. auto. Qed.
+
+Lemma to_list_nth {T n} (xs : vec T n) i
+                  : List.nth_error (to_list xs) (Fin.to_nat i) = Some (v2a xs i).
+Proof. induction xs. inversion i. destruct i; auto. apply IHxs. Qed.
+
+Fixpoint of_list {T : Set} (xs : list T) : vec T (length xs) :=
+match xs as xs' return vec T (length xs') with
+| nil => NilVec
+| cons x xs => ConsVec x (of_list xs)
+end.
+
+End Vec.
